\vbox{\offinterlineskip 
\halign{\tabskip=1em plus 4em \quad$#\hfil$\quad\cr
\noalign{\bf{Basic Algebraic Equations} \hfil} \cr
\noalign{\hrule\vskip 1 mm}
\displaystyle (a \pm b)^2 = a^2 \pm 2ab + b^2 \cr\noalign{\vskip 1mm}
\displaystyle (a \pm b)^3 = a^3 \pm b^3 \pm 3a^2b + 2ab^2 \cr
\noalign{\vskip 1mm}
\displaystyle a^2 - b^2 = (a+b)(a-b) \cr\noalign{\vskip 1mm}
\displaystyle a^3 \pm b^3 = (a \pm b)(a^2 \pm ab + b^2) \cr\noalign{\vskip 1mm}
\displaystyle (a+b+c)^2 = a^2 + b^2 + c^2 + 2ab + 2ac + 2bc \cr
\noalign{\vskip 1mm}
\displaystyle (a+b+c)^3 = a^3 + b^3 + c^3 + 3a^2b + 3ab^2 + 3a^2c + \cr
\noalign{\vskip 1mm}
\omit \hfil $\displaystyle + 3ac^2 + 3bc^2 + 3b^2c + 6abc$ \cr
\noalign{\vskip 1mm \hrule} \cr
}
}
