\vbox{\offinterlineskip
\def\halpha{{\alpha \over 2}}
\halign{\tabskip=1em plus 1em%
\quad$\displaystyle #\hfil$&$\displaystyle #\hfil$\quad\cr
\noalign{\bf{Half-Angle} \hfil \vskip 1mm} \cr
\noalign{\hrule\vskip 1 mm}
\sin\halpha = \sqrt{{1 - \cos\alpha} \over 2} &
\cos\halpha = \sqrt{{1 + \cos\alpha} \over 2} \cr
\noalign{\vskip 1ex}
%
\sin\alpha = {{2\tan\halpha} \over {1 + \tan^2\halpha}} &
\cos\alpha = {{1 - \tan^2\halpha} \over {1 + \tan^2\halpha}} \cr
\noalign{\vskip 1ex}
%
\tan\halpha = \sqrt{{1 - \cos\alpha} \over {1 + \cos\alpha}} &
\tan\alpha = {{2\tan\halpha} \over {1 - \tan^2\halpha}} \cr
\noalign{\vskip 1ex}
%
\omit\quad$\displaystyle %
\tan\halpha = {{\sin\alpha} \over {1 + \cos\alpha}} = %
{{1 - \cos\alpha} \over {\sin\alpha}} %
$\span \quad \cr
\noalign{\vskip 1ex}
%
\omit\quad$\displaystyle %
\cot\halpha = \sqrt{{1 + \cos\alpha} \over {1 - \cos\alpha}} = %
{{1 + \cos\alpha} \over {\sin\alpha}} = %
{{\sin\alpha} \over {1 - \cos\alpha}} %
$\span \quad \cr
\noalign{\vskip 1ex}
%
\omit\quad$\displaystyle %
\tan\alpha\tan\halpha = \sec\alpha - 1 = %
{{1 - \cos\alpha} \over {\cos\alpha}}%
$ \span \quad \cr
\noalign{\vskip 1ex}
%
1 + \sin\alpha = 2\cos^2({\pi \over 4} - \halpha) &
1 + \cos\alpha = 2\cos^2\halpha \cr
\noalign{\vskip 1ex}
%
1 - \sin\alpha = 2\sin^2({\pi \over 4} - \halpha) &
1 - \cos\alpha = 2\sin^2 \halpha \cr
\noalign{\vskip 1ex}
%
1 + \tan\alpha = \sqrt{2}~{{\sin({\pi \over 4} + \alpha)} \over {\cos\alpha}} &
1 - \tan\alpha = \sqrt{2}~{{\sin({\pi \over 4} - \alpha)} \over {\cos\alpha}}\cr
\noalign{\vskip 1ex}
%
\noalign{\vskip 1mm \hrule} \cr
}
}
