\vbox{\offinterlineskip 
\halign{\tabskip=1em plus 4em \quad$#\hfil$&$#\hfil$\quad\cr
\noalign{\bf{Sums of Series} \hfil \vskip 1mm} \cr
\noalign{\hrule\vskip 1 mm}
\displaystyle \sum_{i=1}^n i = {n(n+1) \over 2} & 
\omit In general: \hfil \cr\noalign{\vskip 1mm}
\displaystyle \sum_{i=1}^n i^2 = {n(n+1)(2n+1) \over 6} &
\displaystyle \sum_{i=1}^n i^m = {1 \over m+1} \bigg[ %
     (n+1)^{m+1} - 1 - \cr\noalign{\vskip 1mm}
\displaystyle \sum_{i=1}^n i^3 = {n^2(n+1)^2 \over 4} &
\omit $\hfil\displaystyle     
     - \sum_{i=1}^n \big((i+1)^{m+1} - i^{m+1} - (m+1)i^m\big) %
\bigg]$ \cr\noalign{\vskip 1mm}
& \displaystyle \sum_{i=1}^{n-1} i^m = {1 \over m+1}%
\sum_{k=0}^m {m+1 \choose k} B_k n^{m+1-k}. \cr
\noalign{\vskip 1mm \hrule} \cr
}
}

